recursion

src/pca.lean
@@ -1,22 +1,22 @@
 import data.option.basic
+import tactic
+--import data.real.basic
 
 universe variable u
 
+variables {α : Type u}
+
 class partial_magma (α : Type u) :=
 (mul : α → α → option α)
+infixl ` ⬝ ` := partial_magma.mul
+infix ` ↓= `:50 := λ x y, x = some y
+prefix `↓`:80 := some
 
-@[simp]
-def partial_magma.mmul {α : Type u} [partial_magma α] : option α → option α → option α
-| (some x) (some y) := partial_magma.mul x y
+def partial_magma.mmul [partial_magma α] : option α → option α → option α
+| ↓x ↓y := x ⬝ y
 | none _ := none
 | _ none := none
-infixl ` ⬝ ` := partial_magma.mul
-
-infix ` ↓= `:50 := λ x y, x = some y
-
-
-
-instance pm_mul {α : Type u} [c : partial_magma α] : has_mul (option α) := {mul := @partial_magma.mmul _ c}
+instance pm_mul [c : partial_magma α] : has_mul (option α) := {mul := @partial_magma.mmul _ c}
 
 /- Partial Combinatory Algebra -/
 class pca (α : Type u) extends partial_magma α :=
@@ -27,28 +27,55 @@ class pca (α : Type u) extends partial_magma α :=
 (stot : ∀ x y : α, option.is_some (s ⬝ x * y))
 (s_substitution : ∀ x y z : α, s ⬝ x * y * z = (x ⬝ z) * (y ⬝ z))
 
-def pca.equiv {α : Type u} [partial_magma α] (a b : option α) : Prop := ∀ x, a * x = b * x
+def pca.equiv [partial_magma α] (a b : option α) : Prop := ∀ x : α, a * ↓x = b * ↓x
 infix ` ≃ `:50 := pca.equiv 
 
 namespace pca
 
-variables {α : Type u}
+def const [pca α] (x : α) := option.get (ktot x)
+def subst [pca α] (x y : α) := option.get (stot x y)
+notation `𝐤` := const
+notation `𝐬` := subst
 
-@[simp] lemma k_constant_ [c : pca α] : ∀ x y : α, k ⬝ x * (some y) = some x := c.k_constant
-@[simp] lemma s_substitution_ [c : pca α] : ∀ x y z : α, s ⬝ x * (some y) * (some z) = (x ⬝ z) * (y ⬝ z) := c.s_substitution
+lemma k_constant_ [c : pca α] : ∀ x y : α, k ⬝ x * ↓y = ↓x := c.k_constant
+lemma s_substitution_ [c : pca α] : ∀ x y z : α, s ⬝ x * ↓y * ↓z = (x ⬝ z) * (y ⬝ z) := c.s_substitution
+lemma s_substitution_0 [c : pca α] : ∀ x y z : α, ↓s * ↓x * ↓y * ↓z = (x ⬝ z) * (y ⬝ z) := c.s_substitution
+lemma k_compute [pca α] (x : α) : k ⬝ x = ↓(𝐤 x) := by { unfold const, simp }
+lemma s_compute [pca α] (x y : α) : s ⬝ x * ↓y = ↓(𝐬 x y) := by { unfold subst, simp, refl }
 
-def i [pca α] : α := option.get (stot k k)
 
-@[simp]
+lemma constant_simp [pca α] (a b : α) : 𝐤 a ⬝ b ↓= a :=
+begin
+  have e : (k ⬝ a : option α) = ↓(𝐤 a), { unfold const, simp },
+  calc
+    𝐤 a ⬝ b = k ⬝ a * ↓b : by { rw e, refl }
+    ...     = ↓a           : k_constant _ _
+end
+
+lemma substitution_simp [pca α] (a b c : α) : 𝐬 a b ⬝ c = a ⬝ c * b ⬝ c :=
+begin
+  have e : (s ⬝ a * ↓b : option α) = ↓(𝐬 a b), { unfold subst, simp, refl },
+  calc
+    𝐬 a b ⬝ c = s ⬝ a * ↓b * ↓c : by { rw e, refl }
+    ...       = a ⬝ c * b ⬝ c           : s_substitution _ _ _
+end
+
+def i [pca α] : α := 𝐬 k k
+
 lemma i_ident [pca α] (x : α) : i ⬝ x ↓= x :=
 begin
-  have e : s ⬝ k * (some k) = some i, { unfold i, simp, refl },
   calc
-    i ⬝ x = (s ⬝ k * (some k)) * (some x)        : by { rw e, exact rfl }
-    ...   = k ⬝ x * k ⬝ x                        : by { simp }
-    ...   = k ⬝ x * (some (option.get (ktot x))) : by { simp }
-    ...   = some x                               : by { simp only [k_constant_] }
+    i ⬝ x = (𝐬 k k) ⬝ x       : by { unfold i, }
+    ...   = k ⬝ x * k ⬝ x     : by { simp only [substitution_simp], }
+    ...   = k ⬝ x * (↓(𝐤 x)) : by { unfold const, simp, }
+    ...   = ↓x               : by { simp only [k_constant_], }
 end
+
+@[simp] lemma k_compute0 [pca α] (a : α) : ↓k * ↓a = ↓(𝐤 a) := k_compute a
+@[simp] lemma s_compute0 [pca α] (a b : α) : ↓s * ↓a * ↓b = ↓(𝐬 a b) := s_compute a b
+@[simp] lemma k_simp [pca α] (a b : α) : ↓(𝐤 a) * ↓b = ↓a := constant_simp a b
+@[simp] lemma s_simp [pca α] (a b c : α) : ↓(𝐬 a b) * ↓c = (↓a * ↓c) * (↓b * ↓c) := substitution_simp a b c
+@[simp] lemma i_simp [pca α ] (a : α) : ↓i * ↓a = ↓a := i_ident a
 
 inductive lambda (α : Type u) [pca α]
 | var : ℕ → lambda
@@ -58,20 +85,18 @@ instance lambda_mul (α : Type u) [pca α] : has_mul (lambda α) := ⟨lambda.ap
 
 open lambda
 
-def lam [pca α] : ℕ → lambda α → lambda α
-| x (var y) := if x = y then (com i) else (com k) * var y
-| x (com c) := com k * com c
-| x (l * k) := com s * (lam x l) * (lam x k)
+def lam [pca α] (n : ℕ) :lambda α → lambda α
+| (var m) := if n = m then com i else com k * var m
+| (com c) := com k * com c
+| (l * k) := (com s) * (lam l) * (lam k)
 notation `Λ`x`,` := lam x 
 
-def l_to_pca [pca α] : lambda α → option α
-| (var x) := some k
-| (com c) := some c
-| (l * k) := (l_to_pca l) * (l_to_pca k)
+def code [pca α] : lambda α → option α
+| (var x) := ↓k
+| (com c) := ↓c
+| (l * k) := (code l) * (code k)
 
-instance lambda_to_pca {α : Type u} [pca α] : has_coe (lambda α) (option α) := ⟨l_to_pca⟩ 
-
-lemma lambda_defined [c : pca α] : ∀ (n : ℕ) (e : lambda α), option.is_some (l_to_pca (Λ n, e) : option α)
+lemma lambda_defined [c : pca α] : ∀ (n : ℕ) (e : lambda α), option.is_some (code (Λ n, e) : option α)
 | n (var e) := begin
     cases (eq.decidable n e),
     { have he : (Λ n, (var e) : @lambda _ c) = com k * var e, { simp [lam], intros, contradiction },
@@ -83,33 +108,70 @@ lemma lambda_defined [c : pca α] : ∀ (n : ℕ) (e : lambda α), option.is_som
   end
 | n (com c) := ktot c
 | n (l * m) := begin
-    simp [lam, l_to_pca], 
+    simp [lam, code], 
     let a := option.get (lambda_defined n l),
     let b := option.get (lambda_defined n m),
-    have ha : l_to_pca (Λ n, l) = some a, { simp },
-    have hb : l_to_pca (Λ n, m) = some b, { simp },
+    have ha : code (Λ n, l) = ↓a, { simp },
+    have hb : code (Λ n, m) = ↓b, { simp },
     rw [ha, hb],
     exact stot a b
-  end 
+  end
 
-def dapp [pca α] : lambda α := Λ 0, (Λ 1, (Λ 2, (var 0) * ((var 1) * (var 1)) * (var 2)))
+namespace recursionthm
 
+def d [pca α] : α := option.get (lambda_defined 0 (Λ 1, (var 0 * var 0 * var 1)))
 
-def fixpoint [pca α] : α := option.get (lambda_defined 0 (dapp * (var 0) *(dapp * (var 0))))
-def fixpoint' [pca α] : option α := l_to_pca (Λ 0, dapp * (var 0) *(dapp * (var 0)))
-
-theorem kleene_fixpoint [c : pca α] (f : α) :
-  fixpoint ⬝ f ≃ f * (fixpoint ⬝ f) :=
+lemma dtot [pca α] (f : α) : option.is_some (d ⬝ f) :=
 begin
-  have e : l_to_pca (Λ 0, (dapp * (var 0) * (dapp * (var 0)))) = some (@fixpoint _ c),
-  { unfold fixpoint, simp },
-  intros x,
-  calc
-    fixpoint ⬝ f * x = (l_to_pca (Λ 0, (dapp * (var 0) * (dapp * (var 0))))) * (some f) * x : by { rw e, exact rfl }
-    ...              = (l_to_pca (dapp * (com f) * (dapp * (com f)))) * x : by { simp [lam, l_to_pca],  }
-    ...              = f * fixpoint ⬝ f * x : by sorry
+  have e : d ⬝ f = code (Λ 0, (com f * com f * var 0)),
+  { change (d ⬝ f) with (↓d * ↓f), unfold d, simp [lam, code], },
+  rw e,
+  exact (lambda_defined 0 _),
 end
 
+lemma diagonal [pca α] (f x : α) : d ⬝ f * x = f ⬝ f * x :=
+begin
+  calc
+    d ⬝ f * ↓x = ↓d * ↓f * ↓x                                      :rfl
+    ...       = code (Λ 0, (Λ 1, (var 0 * var 0 * var 1))) * ↓f * ↓x : by { unfold d, simp, }
+    ...       = f ⬝ f * ↓x                                            : by { simp [lam, code], refl, }
+end
+
+def v [pca α] : α := option.get (lambda_defined 0 (Λ 1, (var 0 * (com d * var 1))))
+def n [pca α] : α := option.get (lambda_defined 0 (com d * (com v * var 0)))
+
+theorem recursion [pca α] (f : α) : n ⬝ f ≃ f * (n ⬝ f) :=
+begin
+  intros x,
+  let vf := option.get (lambda_defined 0 (com f * (com d * var 0))),  
+  have hv : ↓v * ↓f ↓= vf, { unfold v, simp [lam, code], },
+  have nf_dvf : ↓n * ↓f = ↓d * ↓vf,
+  { calc
+      ↓n * ↓f = code (Λ 0, (com d * (com v * var 0))) * ↓f : by { unfold n, simp, }
+      ...       = ↓d * ↓vf                                  : by { rw ← hv, simp [lam, code], } },
+  calc
+    n ⬝ f * x = ↓n * ↓f * x          : rfl
+    ...       = ↓d * ↓vf * x         : by { rw nf_dvf, }
+    ...       = ↓vf * ↓vf * x        : diagonal vf x
+    ...       = ↓f * (↓d * ↓vf) * x : by { simp [lam, code], }
+    ...       = ↓f * (↓n * ↓f) * x  : by { rw nf_dvf, }
+end
+
+theorem fixpoint_def [pca α] (f : α) : option.is_some (n ⬝ f) :=
+begin
+  let vf := option.get (lambda_defined 0 (com f * (com d * var 0))),  
+  have hv : ↓v * ↓f = ↓vf, { unfold v, simp [lam, code], },
+  have nf_dvf : n ⬝ f = ↓d * ↓vf,
+  { calc
+      ↓n * ↓f = code (Λ 0, (com d * (com v * var 0))) * ↓f : by { unfold n, simp, }
+      ...       = ↓d * ↓vf                                  : by { rw ← hv, simp [lam, code], } },
+  rw nf_dvf,
+  exact (dtot _)
+end
+
+end recursionthm
+
+def fixpoint [pca α] : α := recursionthm.n
+def recursion  [pca α] (f : α) : fixpoint ⬝ f ≃ f * (fixpoint ⬝ f) := recursionthm.recursion f
 
 end pca
-
